Refinery/Term/Extrinsic/Subst.lean
@@ -1,0 +1,57 @@
+import Refinery.Term.Extrinsic.Typing
+
+namespace Refinery
+
+namespace Term
+
+open HasQuant
+
+variable {φ : Type u} {α : Type v} {ε : Type w} [S : Signature φ α ε]
+
+inductive Deriv? : Ctx? α ε → Var? α ε → Term φ (Ty α) → Type _
+  | valid {e : ε} {Γ : Ctx? α ε} {A : Ty α} {a : Term φ (Ty α)} (D : Γ ⊢[e] a : A) (q : EQuant)
+    (hΓ : q ≤ quant Γ) : Deriv? Γ ⟨A, q, e⟩ a
+  | zero {Γ : Ctx? α ε} (hΓ : Γ.del) (a A e) : Deriv? Γ ⟨A, 0, e⟩ a
+
+notation Γ "⊢?" a ":" v => Deriv? Γ v a
+
+inductive SubstDS (φ) {α ε} [S : Signature φ α ε] : Ctx? α ε → Ctx? α ε → Type _
+  | nil {Γ} (hΓ : Γ.del) : SubstDS φ Γ nil
+  | cons {Γ Γl Γr Δ} {v} {a : Term φ _} (hΓ : Γ.PSSplit Γl Γr)
+    (σ : SubstDS φ Γl Δ) (da : Γr ⊢? a : v) : SubstDS φ Γ (Δ.cons v)
+
+def SubstDS.toSubst {Γ Δ} : SubstDS φ Γ Δ → Subst φ (Ty α)
+  | .nil _, i => .invalid
+  | .cons (a := a) .., 0 => a
+  | .cons _ σ _, i + 1 => σ.toSubst i
+
+instance SubstDS.coeSubst : CoeOut (SubstDS φ Γ Δ) (Subst φ (Ty α)) where
+  coe := SubstDS.toSubst
+
+def SubstDS.leftCtx {Γ Δ} : SubstDS φ Γ Δ → Ctx? α ε
+  | .nil _ => Γ
+  | .cons (Γl := Γl) .. => Γl
+
+def SubstDS.rightCtx {Γ Δ} : SubstDS φ Γ Δ → Ctx? α ε
+  | .nil _ => Γ.erase
+  | .cons (Γr := Γr) .. => Γr
+
+def SubstDS.splitCtx {Γ Δ} : (σ : SubstDS φ Γ Δ) → Γ.PSSplit (σ.leftCtx) (σ.rightCtx)
+  | .nil _ => Γ.erase_right
+  | .cons hΓ .. => hΓ
+
+def SubstDS.head {Γ Δ} : SubstDS φ Γ Δ → Var? α ε
+  | .nil _ => ⟨.unit, 0, ⊥⟩
+  | .cons (v := v) .. => v
+
+def SubstDS.headD {Γ Δ} : (σ : SubstDS φ Γ Δ) → σ.rightCtx ⊢? (σ.toSubst 0) : σ.head
+  | .nil hΓ => .zero (by simp [rightCtx]) _ _ _
+  | .cons _ _ da => da
+
+def SubstDS.tail {Γ Δ} : (σ : SubstDS φ Γ Δ) → SubstDS φ σ.leftCtx Δ.tail
+  | .nil hΓ => .nil hΓ
+  | .cons _ σ _ => σ
+
+-- def SubstDS.wkIn {Γ' Γ Δ} (ρ : Γ'.Wk Γ) : SubstDS φ Γ Δ → SubstDS φ Γ' Δ
+--   | .nil hΓ => .nil (hΓ.wk ρ)
+--   | .cons (a := a) hΓ σ da => .cons (a := a) (hΓ.wk' ρ) (σ.wkIn (hΓ.leftWk' ρ)) sorry
